make some progress

proof/MatchState.v
@@ -26,10 +26,10 @@ Definition correct_perm (p: permission) (n: int): Prop :=
 
 
 Definition match_region_at_ofs (mr:memory_region) (bl_regions : block) (ofs : ptrofs) (m: mem)  : Prop :=
-  (exists vl,  Mem.loadv AST.Mint64 m (Vptr bl_regions ofs) = Some (Vint vl) /\ (start_addr mr) = Vint vl)    /\ (**r start_addr mr = Vint vl*)
-    (exists vl,  Mem.loadv AST.Mint64 m (Vptr bl_regions (Ptrofs.add ofs (Ptrofs.repr 4))) = Some (Vint vl) /\ (block_size mr) = Vint vl) /\ (**r block_size mr = Vint vl*)
-    (exists vl,  Mem.loadv AST.Mint64 m (Vptr bl_regions (Ptrofs.add ofs (Ptrofs.repr 8))) = Some (Vint vl) /\ correct_perm (block_perm mr)  vl) /\ (**r block_perm mr = Vint vl*)
-    (exists vl,  Mem.loadv AST.Mint64 m (Vptr bl_regions (Ptrofs.add ofs (Ptrofs.repr 12))) = Some (Vint vl) /\ (block_ptr mr) = Vint vl).
+  (exists vl,  Mem.loadv AST.Mint32 m (Vptr bl_regions ofs) = Some (Vint vl) /\ (start_addr mr) = Vint vl)    /\ (**r start_addr mr = Vint vl*)
+    (exists vl,  Mem.loadv AST.Mint32 m (Vptr bl_regions (Ptrofs.add ofs (Ptrofs.repr 4))) = Some (Vint vl) /\ (block_size mr) = Vint vl) /\ (**r block_size mr = Vint vl*)
+    (exists vl,  Mem.loadv AST.Mint32 m (Vptr bl_regions (Ptrofs.add ofs (Ptrofs.repr 8))) = Some (Vint vl) /\ correct_perm (block_perm mr)  vl) /\ (**r block_perm mr = Vint vl*)
+    (exists vl,  Mem.loadv AST.Mint32 m (Vptr bl_regions (Ptrofs.add ofs (Ptrofs.repr 12))) = Some (Vint vl) /\ (block_ptr mr) = Vint vl).
 
 Definition size_of_region  := Ptrofs.repr (4 * 4). (* 4 * 32 bits *)
 
@@ -115,8 +115,8 @@ Definition state_struct_def: Ctypes.composite_definition :=
       mpc      : Mem.loadv AST.Mint32 m (Vptr bl_state (Ptrofs.repr 0)) = Some (Vint  (pc_loc st));
       mflags   : Mem.loadv AST.Mint32 m (Vptr bl_state (Ptrofs.repr 4)) = Some (Vint  (int_of_flag (flag st)));
       mregs    : match_registers  (regs_st st) bl_state (Ptrofs.repr 8) m;
-      mrs_num : Mem.loadv AST.Mint32 m (Vptr bl_state (Ptrofs.repr (size_of_regs + 8))) = Some (Vint  (Int.repr (Z.of_nat (mrs_num st))));
-      mem_regs : match_regions (bpf_mrs st) bl_state (Ptrofs.repr (size_of_regs + 12)) m;
+      mrs_num : Mem.loadv AST.Mint32 m (Vptr bl_state (Ptrofs.repr (size_of_regs + 8))) = Some (Vint  (Int.repr (Z.of_nat (DxState.mrs_num st)))) /\ (Z.of_nat(DxState.mrs_num st)) >= 1; (**r at least we have the memory region that corresponds to the input paramters of the interpreter *)
+      mem_regs : match_regions (bpf_mrs st) bl_state (Ptrofs.repr (size_of_regs + 12)) m /\ List.length (bpf_mrs st) = (DxState.mrs_num st); (**r the number of bpf_mrs is exactly the mrs_num *)
       mperm    : Mem.range_perm m bl_state 0 (size_of_state st) Cur Freeable
     }.
 
