benchmark/proof/correct_eval_mem_regions.v
@@ -1,0 +1,104 @@
+From bpf.src Require Import DxIntegers DxValues DxMemRegion DxState DxMonad DxInstructions.
+From Coq Require Import List Lia.
+From compcert Require Import Integers Values Clight Memory.
+Import ListNotations.
+Require Import ZArith.
+
+From bpf.proof Require Import Clightlogic MatchState CorrectRel CommonLemma.
+
+From bpf.benchmark Require Import clightlogicexample.
+
+(**
+static struct memory_region *eval_mem_regions(struct bpf_state* st){
+  return ( *st).mrs;
+}
+
+Print eval_mem_regions.
+eval_mem_regions = 
+fun st : stateM => Some (DxState.eval_mem_regions st, st)
+     : M MyMemRegionsType
+
+*)
+
+Section Eval_mem_regions.
+
+  (** The program contains our function of interest [fn] *)
+  Definition p : Clight.program := prog.
+
+  (* [Args,Res] provides the mapping between the Coq and the C types *)
+  Definition args : list Type := [].
+  Definition res : Type := (MyMemRegionsType:Type).
+
+  (* [f] is a Coq Monadic function with the right type *)
+  Definition f : arrow_type args (M res) := eval_mem_regions.
+
+  Variable state_block: block. (**r a block storing all rbpf state information? *)
+
+  (* [fn] is the Cligth function which has the same behaviour as [f] *)
+  Definition fn: Clight.function := f_eval_mem_regions.
+
+  Definition stateM_correct (st:unit) (v: val) (stm:stateM) (m: Memory.Mem.mem) :=
+    v = Vptr state_block Ptrofs.zero /\ match_state state_block stm m.
+
+  (* [match_arg] relates the Coq arguments and the C arguments *)
+  Definition match_arg_list : DList.t (fun x => x -> val -> stateM -> Memory.Mem.mem -> Prop) ((unit:Type) ::args) :=
+    (DList.DCons stateM_correct
+                (DList.DNil _)).
+
+  (* [match_res] relates the Coq result and the C result *)
+  Definition match_res : res -> val -> stateM -> Memory.Mem.mem -> Prop := fun _ _ _ _ => True.
+
+  Instance correct_function3_eval_mem_regions : correct_function3 p args res f fn (nil) false match_arg_list match_res.
+  Proof.
+    correct_function_from_body.
+    correct_body.
+    (** how to use correct_* *)
+    unfold INV.
+    unfold f.
+    repeat intro.
+    get_invariant_more _st.
+
+    unfold stateM_correct in H1.
+    destruct H1 as (Hv_eq & Hst).
+    destruct Hst.
+    clear minj mpc mflags mregs mperm.
+    destruct mrs_num as (Hmrs_num_ld & Hmrs_num_gt).
+    destruct mem_regs as (mem_regs & Hmem_regions_length).
+    subst v.
+
+    destruct (bpf_mrs st).
+    {
+      simpl in Hmem_regions_length.
+      rewrite <- Hmem_regions_length in Hmrs_num_gt.
+      simpl in Hmrs_num_gt.
+      lia.
+    }
+    destruct mem_regs as (Hmem_regs & _).
+    unfold match_region_at_ofs in Hmem_regs.
+    destruct Hmem_regs as ((vl & Hstart_addr & _) & _).
+    unfold Mem.loadv, size_of_regs in Hstart_addr.
+    simpl in Hstart_addr.
+
+    eexists. exists m, Events.E0.
+
+    repeat split; unfold step2.
+    -
+      apply Smallstep.plus_star.
+      repeat forward_clight.
+
+      Transparent Archi.ptr64.
+      rewrite Ptrofs.add_zero_l.
+      unfold Coqlib.align, AST.Mptr; simpl.
+
+      rewrite Hstart_addr; reflexivity.
+
+      reflexivity.
+      reflexivity.
+    - simpl.
+      constructor.
+      reflexivity.
+  Qed.
+
+End Eval_mem_regions.
+
+Existing Instance correct_function3_eval_mem_regions.
