benchmark/proof/correct_get_immediate.v
@@ -1,0 +1,78 @@
+From bpf.src Require Import DxIntegers DxValues DxMemRegion DxState DxMonad DxInstructions.
+From Coq Require Import List Lia.
+From compcert Require Import Integers Values Clight Memory.
+Import ListNotations.
+Require Import ZArith.
+
+From bpf.proof Require Import Clightlogic MatchState CorrectRel CommonLemma.
+
+From bpf.benchmark Require Import clightlogicexample.
+
+(**
+int get_immediate(unsigned long long ins)
+{
+  return (int) (ins >> 32LLU);
+}
+
+Print get_immediate.
+get_immediate = 
+fun ins : int64_t => returnM (int64_to_sint32 (Int64.shru ins int64_32))
+     : int64_t -> M sint32_t
+*)
+
+Section Get_immediate.
+
+  (** The program contains our function of interest [fn] *)
+  Definition p : Clight.program := prog.
+
+  (* [Args,Res] provides the mapping between the Coq and the C types *)
+  (* Definition Args : list CompilableType := [stateCompilableType].*)
+  Definition args : list Type := [(int64_t:Type)].
+  Definition res : Type := (sint32_t:Type).
+
+  (* [f] is a Coq Monadic function with the right type *)
+  Definition f : arrow_type args (M res) := get_immediate.
+
+  Variable state_block: block. (**r a block storing all rbpf state information? *)
+
+  (* [fn] is the Cligth function which has the same behaviour as [f] *)
+  Definition fn: Clight.function := f_get_immediate.
+
+  (* [match_arg] relates the Coq arguments and the C arguments *)
+  Definition match_arg_list : DList.t (fun x => x -> val -> stateM -> Memory.Mem.mem -> Prop) args :=
+    (DList.DCons (stateless int64_correct)
+                (DList.DNil _)).
+
+  (* [match_res] relates the Coq result and the C result *)
+  Definition match_res : res -> val -> stateM -> Memory.Mem.mem -> Prop := fun x v st m => sint32_correct x v.
+
+  Instance correct_function3_get_immediate : correct_function3 p args res f fn (nil) true match_arg_list match_res.
+  Proof.
+    correct_function_from_body.
+    correct_body.
+    (** how to use correct_* *)
+    unfold INV.
+    unfold f.
+    repeat intro.
+    get_invariant_more _ins.
+
+    unfold stateless, int64_correct in H1.
+    subst v.
+
+    eexists. exists m, Events.E0.
+
+    repeat split; unfold step2.
+    -
+      apply Smallstep.plus_star.
+      repeat forward_clight.
+
+      reflexivity.
+      reflexivity.
+    - simpl.
+      constructor.
+      reflexivity.
+  Qed.
+
+End Get_immediate.
+
+Existing Instance correct_function3_get_immediate.
